cfi/refinementAQ.v
@@ -1,0 +1,430 @@
+Require Import Coq.Bool.Bool.
+Require Import Coq.Classes.SetoidDec.
+Require Import lib.utils.
+Require Import lib.Coqlib.
+Require Import concrete.common.
+Require Import cfi.abstract.
+Require Import cfi.qa.
+Require Import cfi.cfi_rules.
+Require Import symbolic.symbolic.
+Require Coq.Vectors.Vector.
+
+Set Implicit Arguments.
+
+Section Refinement.
+
+Context {mt : machine_types}
+        {ops : machine_ops mt}
+        {opss : machine_ops_spec ops}
+        {ap : Abstract.abstract_params mt}
+        {aps : Abstract.params_spec ap}
+        {sp : @SymbolicCFI.sym_cfi_params mt}.
+
+Variable valid_jmp : word mt -> word mt -> bool.
+
+(* Instantiate the symbolic machine with the CFI stuff*)
+Definition sym_params := SymbolicCFI.sym_cfi valid_jmp.
+
+Context {sps : @Symbolic.params_spec mt sym_params}.
+
+Variable atable : list (Abstract.syscall mt).
+Variable stable : list (@Symbolic.syscall mt sym_params).
+
+(*this should be replaced, when step_a is defined*)
+Variable step_a : @Symbolic.state mt sym_params -> @Symbolic.state mt sym_params -> Prop.
+
+
+Definition amachine := Abstract.abstract_cfi_machine atable valid_jmp.
+Definition smachine := SymbolicCFI.symbolic_cfi_machine stable step_a.
+
+Definition refine_dmemory (admem : Abstract.dmemory mt) (smem : @Symbolic.memory mt sym_params) :=
+  forall w (x : word mt),
+    Symbolic.get_mem smem w = Some x@DATA <->
+    Abstract.get_dmem admem w = Some x. 
+
+Definition refine_imemory (aimem : Abstract.imemory mt) (smem : @Symbolic.memory mt sym_params) :=
+  forall w x,
+    (forall id, Symbolic.get_mem smem w = Some x@(INSTR id) ->
+                Abstract.get_imem aimem w = Some x) /\
+    (exists id, Abstract.get_imem aimem w = Some x ->
+                Symbolic.get_mem smem w = Some x@(INSTR id)).
+
+Definition refine_registers (areg : Abstract.registers mt) (sreg : @Symbolic.registers mt sym_params) :=
+  forall n (x : word mt),
+    (forall ut, Symbolic.get_reg sreg n = Some x@ut ->
+                Abstract.get_reg areg n = Some x) /\
+    (exists ut, Abstract.get_reg areg n = Some x ->
+                Symbolic.get_reg sreg n = Some x@ut).
+
+(*what about syscalls?*)
+Definition refine_normal_state (ast : Abstract.state mt) (sst : Symbolic.state mt) :=
+  let '(Symbolic.State mem regs pc@tpc _) := sst in
+  let '(imem, dmem, aregs, apc, b) := ast in
+  b = true /\
+  pc = apc /\
+  refine_imemory imem mem /\
+  refine_dmemory dmem mem /\
+  refine_registers aregs regs. 
+
+Definition refine_violation_state (ast : Abstract.state mt) (sst : Symbolic.state mt) :=
+  let '(imem, dmem, aregs, apc, b) := ast in
+  b = false /\
+  exists ast0 sst0, 
+    let '(_, _, _, apc0, b0) := ast0 in
+    b0 = true /\
+    Abstract.step atable valid_jmp ast0 ast /\
+    Symbolic.step stable sst0 sst /\
+    refine_normal_state ast0 sst0 /\
+    valid_jmp apc0 apc = false.
+
+Definition refine_state ast sst := 
+  refine_normal_state ast sst \/ refine_violation_state ast sst.
+
+Hypothesis id_hypothesis :
+  forall pc (w : word mt) (mem : @Symbolic.memory mt sym_params) id, 
+    Symbolic.get_mem mem pc = Some w@(INSTR (Some id)) ->
+    id = pc.
+
+Hypothesis jump_tagged :
+  forall pc w smem aimem r,
+    Abstract.get_imem aimem pc = Some w ->
+    decode_instr w = Some (Jump _ r) ->
+    refine_imemory aimem smem ->
+    Symbolic.get_mem smem pc = Some w@(INSTR (Some pc)).
+
+Hypothesis jal_tagged :
+  forall pc w smem aimem r,
+    Abstract.get_imem aimem pc = Some w ->
+    decode_instr w = Some (Jal _ r) ->
+    refine_imemory aimem smem ->
+    Symbolic.get_mem smem pc = Some w@(INSTR (Some pc)).
+
+
+Import Vector.VectorNotations.
+
+Lemma refine_registers_upd sreg sreg' areg r v t v' t' :
+  refine_registers areg sreg ->
+  Symbolic.get_reg sreg r = Some v@t ->
+  Symbolic.upd_reg sreg r v'@t' = Some sreg' ->
+  exists areg',
+    Abstract.upd_reg areg r v' = Some areg' /\
+    refine_registers areg' sreg'.
+Proof.
+  intros REFR GET UPD. unfold refine_registers in REFR.
+  destruct (REFR r v) as [REGSA REGAS].
+  apply REGSA in GET.
+  assert (NEW := PartMaps.upd_defined v' GET).
+  destruct NEW as [areg' UPD'].
+  eexists; split; eauto.
+  unfold refine_registers. intros r' v''.
+  destruct (r' == r) as [EQ | NEQ]; [simpl in EQ | simpl in NEQ]; subst.
+  *
+    rewrite (PartMaps.get_upd_eq UPD').
+    rewrite (PartMaps.get_upd_eq UPD). 
+    split. 
+    - intros ut H. inversion H; reflexivity.
+    - exists t'. intro H1; inversion H1; auto.
+  * rewrite (PartMaps.get_upd_neq NEQ UPD).
+    rewrite (PartMaps.get_upd_neq NEQ UPD').
+    auto.
+Qed.
+
+Lemma refine_memory_upd smem smem' amemd addr v v' :
+  refine_dmemory amemd smem ->
+  Symbolic.get_mem smem addr = Some v@DATA ->
+  Symbolic.upd_mem smem addr v'@DATA = Some smem' ->
+  exists amemd',
+    Abstract.upd_dmem amemd addr v' = Some amemd' /\
+    refine_dmemory amemd' smem'.
+Proof.
+  intros MEM GET UPD. unfold refine_dmemory in MEM.
+  assert (GET': Abstract.get_dmem amemd addr = Some v) 
+    by (apply MEM in GET; auto).
+  destruct (PartMaps.upd_defined v' GET') as [amem' UPD'].
+  do 2 eexists; eauto.
+  intros addr' w'.
+  destruct (addr' == addr) as [EQ | NEQ]; [simpl in EQ | simpl in NEQ]; subst.
+  - rewrite (PartMaps.get_upd_eq UPD).
+    rewrite (PartMaps.get_upd_eq UPD').
+    split; try congruence.
+  - rewrite (PartMaps.get_upd_neq NEQ UPD').
+    rewrite (PartMaps.get_upd_neq NEQ UPD).
+    now apply MEM.
+Qed.
+
+Lemma data_memory_upd (smem : @Symbolic.memory mt sym_params) smem' addr v v' :
+  Symbolic.get_mem smem addr = Some v@DATA -> 
+  Symbolic.upd_mem smem addr v'@DATA = Some smem' ->
+  (forall addr' i id, 
+     Symbolic.get_mem smem addr' = Some i@(INSTR id) ->
+     Symbolic.get_mem smem' addr' = Some i@(INSTR id)).
+Proof.
+  intros GET UPD addr' i id GET'.
+  destruct (addr' == addr) as [EQ | NEQ]; [simpl in EQ | simpl in NEQ]; subst.
+  * rewrite GET in GET'. discriminate.
+  * rewrite (PartMaps.get_upd_neq NEQ UPD);
+    assumption.
+Qed.
+
+Lemma imem_upd_preservation amemi (smem : @Symbolic.memory mt sym_params) (smem' : @Symbolic.memory mt sym_params) addr v v':
+  refine_imemory amemi smem ->
+  Symbolic.get_mem smem addr = Some v@DATA ->
+  Symbolic.upd_mem smem addr v'@DATA = Some smem' ->
+  refine_imemory amemi smem'.
+Proof.
+  intros MEM GET UPD w x.
+  destruct (MEM w x) as [MEMSA MEMAS].
+  split.
+  - intros id GET'.
+    destruct (addr == w) as [EQ | NEQ]; [simpl in EQ | simpl in NEQ]; subst.
+    * assert (CONTRA := PartMaps.get_upd_eq UPD).
+      rewrite CONTRA in GET'. discriminate.
+    * eapply PartMaps.get_upd_neq in UPD; eauto.
+      Focus 2. apply sps.
+      rewrite UPD in GET'.
+      eapply MEMSA; eauto.
+  - destruct MEMAS as [id' H].
+    exists id'.
+    intro GET'. apply H in GET'.
+    destruct (addr == w) as [EQ | NEQ]; [simpl in EQ | simpl in NEQ]; subst.
+    * rewrite GET in GET'. discriminate.
+    * eapply PartMaps.get_upd_neq in UPD; eauto. Focus 2. apply sps.
+      rewrite UPD; assumption.
+Qed.
+
+Hint Resolve imem_upd_preservation.
+
+Ltac match_inv :=
+  repeat match goal with
+  | H : bind (fun x : _ => _) _ = Some _ |- _ =>
+    apply bind_inv in H;
+    let x := fresh x in
+    let E := fresh "E" in
+    destruct H as (x & H & E);
+    simpl in H; simpl in E
+  | H : (if ?b then _ else _) = Some _ |- _ =>
+    let E := fresh "E" in
+    destruct b eqn:E;
+    try discriminate
+  | H : match ?E with _ => _ end = _ |- _ =>
+    destruct E eqn:?; try discriminate
+  | H : Some _ = Some _ |- _ => inv H
+  | H : ?O = Some _ |- context[bind _ ?O] => rewrite H; simpl
+  | H : True |- _ => clear H
+  end.
+
+Theorem backwards_simulation_normal ast sst sst' :
+  refine_normal_state ast sst ->
+  Symbolic.step stable sst sst' ->
+  exists ast',
+    Abstract.step atable valid_jmp ast ast' /\
+    refine_state ast' sst'.
+Proof.
+  intros REF SSTEP.
+  destruct ast as [[[[imem dmem] aregs] apc] b].
+  destruct b; [idtac | inversion SSTEP; subst; destruct REF; discriminate].
+  inversion SSTEP; subst;
+  destruct REF as [? [? [? [? ?]]]]; subst apc;
+  (*unfoldings and case analysis on tags*)
+  repeat (
+      match goal with
+        | [H: Symbolic.next_state_pc _ _ _ = _ |- _] => unfold Symbolic.next_state_pc in H
+        | [H: Symbolic.next_state_reg _ _ _ _ = _ |- _] => unfold Symbolic.next_state_reg in H
+        | [H: Symbolic.next_state_reg_and_pc _ _ _ _ _ = _ |- _] => 
+          unfold Symbolic.next_state_reg_and_pc in H
+        | [H: Symbolic.next_state _ _ _ = Some _ |- _] =>
+          unfold Symbolic.next_state in H; simpl in H; match_inv
+      end);
+  (* switch memory updates to abstract*)
+  repeat (
+      match goal with
+        | [H: SymbolicCFI.upd_mem ?Mem ?Addr ?V@_ = Some _, H1 : refine_dmemory _ ?Mem, 
+          H2: Symbolic.get_mem ?Mem ?Addr = Some _ |- _] => 
+          simpl in H; destruct (refine_memory_upd Addr V H1 H2 H) as [dmem' [? ?]]
+  end);
+
+  (*switch memory and register reads to abstract*)
+  repeat  match goal with
+    | [H1: refine_imemory _ _, H2: Symbolic.get_mem _ _ = Some _@(INSTR _) |- _] =>
+      apply H1 in H2
+    | [H1: refine_dmemory _ _, H2: Symbolic.get_mem _ _ = Some _@DATA |- _] => 
+      apply H1 in H2
+    | [H1: refine_registers _ _, H2: Symbolic.get_reg _ _ = Some _ |- _] => 
+      apply H1 in H2
+  end;
+        
+  repeat match goal with
+    | [H: refine_registers ?Aregs ?Regs, H1: Abstract.get_reg _ ?R = Some ?Old |- _] => 
+      unfold refine_registers in H; destruct (H R Old) as [RSA RAS]; destruct RAS as [x RAS'];
+      apply RAS' in H1; fold (refine_registers Aregs Regs) in H
+    | [H: refine_registers _ _, H1: Symbolic.get_reg ?Reg ?R = Some _,
+                                    H2: SymbolicCFI.upd_reg _ ?R ?V'@?T' = Some _ |- _] =>
+      destruct (refine_registers_upd R V' T' H H1 H2) as [aregs' [? ?]]
+    
+  end; auto;
+
+  (*handle abstract steps*)
+  repeat (match goal with 
+    | [|- exists _,  _ /\ _] => eexists; split
+    | [|- Abstract.step _ _ _ _] => econstructor(eassumption)
+    | [H: decode_instr _ = Some (Load _ _ _) |- Abstract.step _ _ _ _] => 
+      eapply Abstract.step_load; eauto
+    | [H: Symbolic.get_mem _ ?Addr = _, H1: refine_imemory _ _, H2: refine_dmemory _ _ 
+       |- Abstract.get_imem _ ?Addr =  _ \/ Abstract.get_dmem _ ?Addr = _] => (*for load*)
+      destruct t2; [left; apply H1 in H; eassumption | right; apply H2 in H; eassumption]
+    | [H: decode_instr _ = Some (Store _ _ _) |- Abstract.step _ _ _ _] => 
+      eapply Abstract.step_store; eauto
+    | [H: decode_instr _ = Some (Jump _ _ ) |- Abstract.step _ _ _ _] => 
+      eapply Abstract.step_jump; eauto
+    | [H: decode_instr _ = Some (Bnz _ _ _) |- Abstract.step _ _ _ _] =>
+      eapply Abstract.step_bnz; eauto
+    | [H: decode_instr _ = Some (Jal _ _ ) |- Abstract.step _ _ _ _] =>
+      eapply Abstract.step_jal; eauto
+         end);
+
+  (*handle final state refinement*)
+  repeat (match goal with
+    | [H: decode_instr _ = Some (Jump _ _) |- refine_state (_,_,_,_, valid_jmp ?Pc ?W) _] =>
+      remember (valid_jmp Pc W) as b; destruct b; [left; unfold refine_normal_state; repeat (split; auto) | idtac]
+    | [H: false = valid_jmp ?Pc ?W |- refine_state (_,_,_,_, false) _] =>
+      right; unfold refine_violation_state
+    | [|- _ /\ _] => split; [eauto | idtac]
+    | [|- exists _ _, _] => exists (imem,dmem,aregs,pc,true)
+    | [|- exists _, _] => eexists
+    | [H: decode_instr _ = Some (Jump _ _) |- Abstract.step _ _ _ (_,_,_,_,false)] =>
+      eapply Abstract.step_jump; eauto
+    | [|- refine_state (_,_,_,_,true) _] => left 
+    | [|- refine_normal_state _ _] => unfold refine_normal_state; simpl
+    | [H: refine_imemory ?Imem ?Mem |- refine_imemory ?Imem ?Mem] => assumption
+    | [H: refine_imemory ?Imem ?Mem |- refine_imemory ?Imem ?Mem'] => 
+        eapply imem_upd_preservation; eauto
+   end); 
+  repeat match goal with
+           | [H: refine_dmemory dmem ?Mem |- Symbolic.get_mem ?Mem _ = Some _] => eapply H; eauto
+         end; auto. 
+
+(*TODO: SYSTEM CALLS*)
+Admitted.           
+
+Lemma imem_refined_instructions mem imem pc i i' ut :
+  refine_imemory imem mem ->
+  Abstract.get_imem imem pc = Some i ->
+  Symbolic.get_mem mem pc = Some i'@ut ->
+  decode_instr i = decode_instr i'.
+Proof.
+  intros MEM GET GET'.
+  destruct (MEM pc i).
+  destruct H0. apply H0 in GET. rewrite GET in GET'. inversion GET'. subst. reflexivity.
+Qed.
+
+Lemma reg_refined_values reg areg r v v' ut :
+  refine_registers areg reg ->
+  Abstract.get_reg areg r = Some v ->
+  Symbolic.get_reg reg r = Some v'@ut ->
+  v = v'.
+Proof.
+  intros REG GET GET'.
+  destruct (REG r v). destruct H0. apply H0 in GET.
+  rewrite GET in GET'. inversion GET'. reflexivity.
+Qed.
+
+
+Theorem backwards_simulation_violation ast sst sst' :
+  refine_violation_state ast sst ->
+  Symbolic.step stable sst sst' ->
+  exists ast',
+    Abstract.step atable valid_jmp ast ast' /\
+    refine_state ast' sst'.
+Proof.
+  intros REF SSTEP.
+  destruct ast as [[[[imem dmem] aregs] apc] b].
+  destruct b; [inversion SSTEP; subst; destruct REF; discriminate | idtac];
+  inversion SSTEP; subst.
+  (*nop*)
+  unfold refine_violation_state in REF.
+  destruct REF as [? [ast0 [sst0 REF]]].
+  destruct ast0 as [[[[imem0 dmem0] aregs0] apc0] b0].
+  destruct REF as [? [? [? [? ?]]]]; subst.
+  unfold Symbolic.next_state_pc in NEXT. unfold Symbolic.next_state in NEXT.
+  simpl in NEXT.
+  unfold refine_normal_state in H3. 
+  destruct sst0 as [mem0 regs0 [pc0 tpc0] ?]. 
+  destruct H3 as [? [? [? [? ?]]]].
+  inversion H1; subst.
+  * (*case amachine took a jump*)
+    inversion H2; inversion ST; subst;
+    (*uninteresting cases*)
+    match goal with 
+        | [H: refine_imemory ?Imem ?Mem, H1: Abstract.get_imem ?Imem ?Pc = Some ?I,
+           H2: Symbolic.get_mem ?Mem ?Pc = Some ?I'@_ |- _] => 
+          destruct (imem_refined_instructions Pc H H1 H2); try congruence
+    end. 
+    (*case smachine took a jump too*)
+    unfold Symbolic.next_state_pc in NEXT0.
+    unfold Symbolic.next_state in NEXT0. simpl in NEXT0.
+    assert (GET := jump_tagged pc0 FETCH INST0 H5). 
+    assert (ti0 = (INSTR (Some pc0))).
+    { rewrite GET in PC0. inversion PC0; auto. }
+    subst ti0.
+    destruct tpc1.
+    { (*case sst0 has a pc tag set*)
+      destruct o; [idtac | inversion NEXT0].
+      destruct (valid_jmp w0 pc0); [idtac | inversion NEXT0].
+      simpl in NEXT0. inversion NEXT0; subst.
+      destruct ti. (*could avoid this*)
+      - (*case ti is tagged as an instr*)
+        destruct o.
+        + (*case ti has an id - only valid case since we are coming from a jump*)
+          assert (w = pc) by (eapply id_hypothesis; eauto). subst w.
+          assert (r = r0) by (rewrite INST0 in INST1; inversion INST1; auto); subst r0.
+          assert (EQ := reg_refined_values r H7 RW RW0). subst apc.
+          rewrite VALID in NEXT. simpl in NEXT. inversion NEXT.
+        + simpl in NEXT; inversion NEXT.
+      - simpl in NEXT; inversion NEXT.
+    }
+    { simpl in NEXT0. inversion NEXT0; subst.
+      destruct ti. (*could avoid this*)
+      - (*case ti is tagged as an instr*)
+        destruct o.
+        + (*case ti has an id - only valid case since we are coming from a jump*)
+          assert (w = pc) by (eapply id_hypothesis; eauto). subst w.
+          assert (r = r0) by (rewrite INST0 in INST1; inversion INST1; auto); subst r0.
+          assert (EQ := reg_refined_values r H7 RW RW0). subst apc.
+          rewrite VALID in NEXT. simpl in NEXT. inversion NEXT.
+        + simpl in NEXT; inversion NEXT.
+      - simpl in NEXT; inversion NEXT.
+    }
+  * (*case amachine took a JAL*)
+    inversion H2; inversion ST; subst;
+    (*uninteresting cases*)
+    match goal with 
+        | [H: refine_imemory ?Imem ?Mem, H1: Abstract.get_imem ?Imem ?Pc = Some ?I,
+           H2: Symbolic.get_mem ?Mem ?Pc = Some ?I'@_ |- _] => 
+          destruct (imem_refined_instructions Pc H H1 H2); try congruence
+    end.
+    
+      
+
+(* ast ~v sst,  ast = (imem,dmem,reg,apc,false) 
+   sst -> sst'
+  --------------------
+   ast ~v sst => ast0 ~ sst0, ast0 -> ast, sst0 -> sst, valid_jmp apc0 apc = false
+   
+   1. analysis on sst -> sst'
+      a. case tpc = INSTR (Some n) and ti = INTR (Some m). By hypothesis n = apc0, m = apc.
+      b. case tpc = DATA. by SSTEP, sst' rvec results in INSTR. Contadiction.
+    
+
+*)
+
+Theorem backwards_simulation ast sst sst' :
+  refine_state ast sst ->
+  Symbolic.step stable sst sst' ->
+  exists ast',
+    Abstract.step atable valid_jmp ast ast' /\
+    refine_state ast' sst'.
+Proof.
+Admitted.
+ 
+    
+    
